Verify saturn/spmc_future.

theories/saturn/spmc_future.v
@@ -1,7 +1,11 @@
 From zebre Require Import
   prelude.
+From zebre.iris.base_logic Require Import
+  lib.oneshot
+  lib.excl.
 From zebre.language Require Import
-  notations.
+  notations
+  diaframe.
 From zebre.std Require Import
   opt
   condition.
@@ -9,6 +13,10 @@ From zebre.saturn Require Export
   base.
 From zebre Require Import
   options.
+
+Implicit Types b : bool.
+Implicit Types l : location.
+Implicit Types o : option val.
 
 #[local] Notation "'result'" := (
   in_type "t" 0
@@ -38,6 +46,7 @@ Definition spmc_future_set : val :=
 Definition spmc_future_try_get : val :=
   λ: "t",
     "t".{result}.
+
 Definition spmc_future_get : val :=
   λ: "t",
     match: spmc_future_try_get "t" with
@@ -48,10 +57,297 @@ Definition spmc_future_get : val :=
         let: "cond" := "t".{condition} in
         mutex_protect "mtx" (λ: <>,
           condition_wait_while "cond" "mtx" (λ: <>, "t".{result} = §None)
-        )
+        ) ;;
+        let: ‘Some "v" := "t".{result} in
+        "v"
     end.
+
+Class SpmcFutureG Σ `{zebre_G : !ZebreG Σ} := {
+  #[local] spmc_future_G_mutex_G :: MutexG Σ ;
+  #[local] spmc_future_G_lstate_G :: OneshotG Σ unit val ;
+}.
+
+Definition spmc_future_Σ := #[
+  mutex_Σ ;
+  oneshot_Σ unit val
+].
+#[global] Instance subG_spmc_future_Σ Σ `{zebre_G : !ZebreG Σ} :
+  subG spmc_future_Σ Σ →
+  SpmcFutureG Σ .
+Proof.
+  solve_inG.
+Qed.
+
+Section spmc_future_G.
+  Context `{spmc_future_G : SpmcFutureG Σ}.
+
+  #[local] Definition spmc_future_inv_inner l γ Ψ : iProp Σ :=
+    ∃ o,
+    l.[result] ↦ o ∗
+    match o with
+    | Some v =>
+        oneshot_shot γ v ∗
+        □ Ψ v
+    | None =>
+        oneshot_pending γ (DfracOwn (1/3)) ()
+    end.
+  Definition spmc_future_inv t Ψ : iProp Σ :=
+    ∃ l γ mtx cond,
+    ⌜t = #l⌝ ∗
+    meta l nroot γ ∗
+    l.[mutex] ↦□ mtx ∗
+    mutex_inv mtx True ∗
+    l.[condition] ↦□ cond ∗
+    condition_inv cond ∗
+    inv nroot (spmc_future_inv_inner l γ Ψ).
+
+  Definition spmc_future_producer t : iProp Σ :=
+    ∃ l γ,
+    ⌜t = #l⌝ ∗
+    meta l nroot γ ∗
+    oneshot_pending γ (DfracOwn (2/3)) ().
+
+  Definition spmc_future_result t v : iProp Σ :=
+    ∃ l γ,
+    ⌜t = #l⌝ ∗
+    meta l nroot γ ∗
+    oneshot_shot γ v.
+
+  #[global] Instance spmc_future_inv_contractive t n :
+    Proper ((pointwise_relation _ (dist_later n)) ==> (≡{n}≡)) (spmc_future_inv t).
+  Proof.
+    rewrite /spmc_future_inv /spmc_future_inv_inner. solve_contractive.
+  Qed.
+  #[global] Instance spmc_future_inv_proper t :
+    Proper ((pointwise_relation _ (≡)) ==> (≡)) (spmc_future_inv t).
+  Proof.
+    intros Ψ1 Ψ2 HΨ.
+    apply equiv_dist => n.
+    apply spmc_future_inv_contractive => v.
+    dist_later_intro.
+    apply equiv_dist, HΨ.
+  Qed.
+
+  #[global] Instance spmc_future_inv_persistent t Ψ :
+    Persistent (spmc_future_inv t Ψ).
+  Proof.
+    apply _.
+  Qed.
+  #[global] Instance spmc_future_result_persistent t v :
+    Persistent (spmc_future_result t v).
+  Proof.
+    apply _.
+  Qed.
+  #[global] Instance spmc_future_producer_timeless t :
+    Timeless (spmc_future_producer t).
+  Proof.
+    apply _.
+  Qed.
+  #[global] Instance spmc_future_result_timeless t v :
+    Timeless (spmc_future_result t v).
+  Proof.
+    apply _.
+  Qed.
+
+  Lemma spmc_future_producer_exclusive t :
+    spmc_future_producer t -∗
+    spmc_future_producer t -∗
+    False.
+  Proof.
+    iIntros "(%l & %γ & -> & #Hmeta & Hpending1) (%_l & %_γ & %Heq & _Hmeta & Hpending2)". injection Heq as <-.
+    iDestruct (meta_agree with "Hmeta _Hmeta") as %<-. iClear "_Hmeta".
+    iDestruct (oneshot_pending_valid_2 with "Hpending1 Hpending2") as %(? & _). done.
+  Qed.
+
+  Lemma spmc_future_create_spec Ψ :
+    {{{ True }}}
+      spmc_future_create ()
+    {{{ t,
+      RET t;
+      spmc_future_inv t Ψ ∗
+      spmc_future_producer t
+    }}}.
+  Proof.
+    iIntros "%Φ _ HΦ".
+
+    wp_rec.
+    wp_smart_apply (mutex_create_spec True with "[//]") as "%mtx #Hmtx_inv".
+    wp_smart_apply (condition_create_spec _ with "[//]") as "%cond #Hcond_inv".
+    wp_record l as "Hmeta" "(Hresult & Hmtx & Hcond & _)".
+    iMod (pointsto_persist with "Hmtx") as "Hmtx".
+    iMod (pointsto_persist with "Hcond") as "Hcond".
+
+    iMod (oneshot_alloc ()) as "(%γ & Hpending)".
+    iEval (assert (1 = 2/3 + 1/3)%Qp as -> by compute_done) in "Hpending".
+    iDestruct "Hpending" as "(Hpending1 & Hpending2)".
+
+    iMod (meta_set _ _ γ with "Hmeta") as "#Hmeta"; first done.
+
+    iSteps. iExists None. iSteps.
+  Qed.
+
+  Lemma spmc_future_set_spec t Ψ v :
+    {{{
+      spmc_future_inv t Ψ ∗
+      spmc_future_producer t ∗
+      □ Ψ v
+    }}}
+      spmc_future_set t v
+    {{{
+      RET ();
+      spmc_future_result t v
+    }}}.
+  Proof.
+    iIntros "%Φ ((%l & %γ & %mtx & %cond & -> & #Hmeta & #Hmtx & #Hmtx_inv & #Hcond & #Hcond_inv & #Hinv) & (%_l & %_γ & %Heq & _Hmeta & Hpending) & HΨ) HΦ". injection Heq as <-.
+    iDestruct (meta_agree with "Hmeta _Hmeta") as %<-. iClear "_Hmeta".
+
+    wp_rec.
+    wp_pures.
+
+    wp_bind (_ <- _)%E.
+    iInv "Hinv" as "(%o & Hresult & Ho)".
+    wp_store.
+    destruct o.
+    { iDestruct "Ho" as "(Hshot & _)".
+      iDestruct (oneshot_pending_shot with "Hpending Hshot") as %[].
+    }
+    iCombine "Hpending Ho" as "Hpending".
+    assert (2/3 + 1/3 = 1)%Qp as -> by compute_done.
+    iMod (oneshot_update_shot with "Hpending") as "#Hshot".
+    iSplitR "HΦ". { iExists (Some _). iSteps. }
+    iModIntro.
+
+    wp_load.
+    wp_apply (condition_signal_spec with "Hcond_inv").
+    iSteps.
+  Qed.
+
+  Lemma spmc_future_try_get_spec_result t Ψ v :
+    {{{
+      spmc_future_inv t Ψ ∗
+      spmc_future_result t v
+    }}}
+      spmc_future_try_get t
+    {{{
+      RET Some v : val;
+      Ψ v
+    }}}.
+  Proof.
+    iIntros "%Φ ((%l & %γ & %mtx & %cond & -> & #Hmeta & #Hmtx & #Hmtx_inv & #Hcond & #Hcond_inv & #Hinv) & (%_l & %_γ & %Heq & _Hmeta & #Hshot)) HΦ". injection Heq as <-.
+    iDestruct (meta_agree with "Hmeta _Hmeta") as %<-. iClear "_Hmeta".
+
+    wp_rec.
+    wp_pures.
+
+    iInv "Hinv" as "(%o & Hresult & Ho)".
+    wp_load.
+    destruct o; last first.
+    { iDestruct (oneshot_pending_shot with "Ho Hshot") as %[]. }
+    iDestruct "Ho" as "(_Hshot & #HΨ)".
+    iDestruct (oneshot_shot_agree with "Hshot _Hshot") as %<-. iClear "_Hshot".
+    iSplitR "HΦ". { iExists (Some _). iSteps. }
+    iSteps.
+  Qed.
+  Lemma spmc_future_try_get_spec t Ψ :
+    {{{
+      spmc_future_inv t Ψ
+    }}}
+      spmc_future_try_get t
+    {{{ o,
+      RET o : val;
+      from_option Ψ True o
+    }}}.
+  Proof.
+    iIntros "%Φ (%l & %γ & %mtx & %cond & -> & #Hmeta & #Hmtx & #Hmtx_inv & #Hcond & #Hcond_inv & #Hinv) HΦ".
+
+    wp_rec.
+    wp_pures.
+
+    iInv "Hinv" as "(%o & Hresult & Ho)".
+    wp_load.
+    destruct o as [v |].
+
+    - iDestruct "Ho" as "(Hshot & #HΨ)".
+      iSplitR "HΦ". { iExists (Some _). iSteps. }
+      iModIntro.
+
+      iApply ("HΦ" $! (Some _) with "HΨ").
+
+    - iSplitR "HΦ". { iExists None. iSteps. }
+      iModIntro.
+
+      iApply ("HΦ" $! None).
+      iSteps.
+  Qed.
+
+  Lemma spmc_future_get_spec t Ψ :
+    {{{
+      spmc_future_inv t Ψ
+    }}}
+      spmc_future_get t
+    {{{ v,
+      RET v;
+      Ψ v
+    }}}.
+  Proof.
+    iIntros "%Φ #Hinv HΦ".
+
+    wp_rec.
+    wp_apply (spmc_future_try_get_spec with "Hinv") as ([]) "HΨ"; first iSteps.
+    iClear "HΨ".
+
+    iDestruct "Hinv" as "(%l & %γ & %mtx & %cond & -> & #Hmeta & #Hmtx & #Hmtx_inv & #Hcond & #Hcond_inv & #Hinv)".
+
+    do 2 wp_load.
+    pose (Ψ_mtx (_ : val) := (
+      ∃ v,
+      oneshot_shot γ v
+    )%I).
+    wp_smart_apply (mutex_protect_spec Ψ_mtx with "[$Hmtx_inv]") as (w) "(%v & #Hshot)".
+    { iIntros "Hmtx_locked _".
+      pose (Ψ_cond b := (
+        if b then
+          True
+        else
+          ∃ v,
+          oneshot_shot γ v
+      )%I).
+      wp_smart_apply (condition_wait_while_spec Ψ_cond with "[$Hcond_inv $Hmtx_inv $Hmtx_locked]"); last auto.
+
+      iStep. clear. iIntros "!> %Φ (Hmtx_locked & _) HΦ".
+      wp_pures.
+
+      wp_bind (!_)%E.
+      iInv "Hinv" as "(%o & Hresult & Ho)".
+      wp_load.
+      destruct o as [v |].
+
+      - iDestruct "Ho" as "(#Hshot & HΨ)"; last first.
+        iSplitR "Hmtx_locked HΦ". { iExists (Some _). iSteps. }
+        iSteps.
+
+      - iSplitR "Hmtx_locked HΦ". { iExists None. iSteps. }
+        iSteps.
+    }
+    wp_pures.
+
+    wp_bind (!_)%E.
+    iInv "Hinv" as "(%o & Hresult & Ho)".
+    wp_load.
+    destruct o; last first.
+    { iDestruct (oneshot_pending_shot with "Ho Hshot") as %[]. }
+    iDestruct "Ho" as "(_Hshot & #HΨ)".
+    iDestruct (oneshot_shot_agree with "Hshot _Hshot") as %<-. iClear "_Hshot".
+    iSplitR "HΦ". { iExists (Some _). iSteps. }
+    iSteps.
+  Qed.
+End spmc_future_G.
 
 #[global] Opaque spmc_future_create.
 #[global] Opaque spmc_future_set.
 #[global] Opaque spmc_future_try_get.
 #[global] Opaque spmc_future_get.
+
+#[global] Opaque spmc_future_inv.
+#[global] Opaque spmc_future_producer.
+#[global] Opaque spmc_future_result.
